在 $f_1$ 内叠加 $1$ 相当于 PSS 末尾添加 $(0, 0)$.

| Beta           | Ordinal | PSS                  | 
|:---------------|--------:|:---------------------|
| $f_1(∘, ∘, ∘)$ |     $0$ | $\varnothing$        |
| $f_1(1, ∘, ∘)$ |     $1$ | $(0, 0)$             |
| $f_1(1, 1, ∘)$ |     $2$ | $(0, 0)(0, 0)$       |
| $f_1(1, 1, 1)$ |     $3$ | $(0, 0)(0, 0)(0, 0)$ |

在 $f_1$ 内叠加 $f_2(1)$ 相当于 PSS 末尾添加 $(0, 0)(0, 1)$.

| Beta                         | Ordinal | PSS                        | 
|:-----------------------------|:--------|:---------------------------|
| $f_1(f_2(1), ∘, ∘)$          | $ω$     | $(0, 0)(0, 1)$             |
| $f_1(f_2(1), 1, ∘)$          | $ω+1$   | $(0, 0)(0, 1)(0, 0)$       |
| $f_1(f_2(1), 1, 1)$          | $ω+2$   | $(0, 0)(0, 1)(0, 0)(0, 0)$ |
| $f_1(f_2(1))$                | $ω$     | $(0, 0)(0, 1)$             |
| $f_1(f_2(1)), f_2(1)$        | $ω×2$   | $(0, 0)(0, 1)(0, 0)(0, 1)$ |
| $f_1(f_2(1), f_2(1),f_2(1))$ | $ω×3$   | $(0, 0)(0, 1)(0, 0)(0, 1)$ |
| $f_1(f_2(1, 1))$             | $ω^2$   | $(0, 0)(1, 0)(1, 0)$       |

在 $f_2$ 内叠加 $1$ 相当于 PSS 末尾添加 $(0, 1)$.

| Beta           | Ordinal | PSS                        |
|:---------------|--------:|:---------------------------|
| $f_2(∘, ∘, ∘)$ |     $1$ | $(0, 0)$                   |
| $f_2(1, ∘, ∘)$ |     $ω$ | $(0, 0)(0, 1)$             |
| $f_2(1, 1, ∘)$ |   $ω^2$ | $(0, 0)(0, 1)(0, 1)$       |
| $f_2(1, 1, 1)$ |   $ω^3$ | $(0, 0)(0, 1)(0, 1)(0, 1)$ |

在 $f_2$ 内叠加 $f_2(1)$ 相当于 PSS 末尾添加 $(n, 0)$.

| Beta                |   Ordinal | PSS                              |
|:--------------------|----------:|:---------------------------------|
| $f_2(f_2(1), ∘, ∘)$ |     $ω^ω$ | $(0, 0)(1, 0)(2, 0)$             |
| $f_2(f_2(1), 1, ∘)$ | $ω^{ω+1}$ | $(0, 0)(1, 0)(2, 0)(1, 0)$       |
| $f_2(f_2(1), 1, 1)$ | $ω^{ω+2}$ | $(0, 0)(1, 0)(2, 0)(1, 0)(1, 0)$ |
| $f_2(f_2(1, 1, ∘))$ | $ω^{ω^2}$ | $(0, 0)(1, 0)(2, 0)(2, 0)$       |
| $f_2(f_2(1, 1, 1))$ | $ω^{ω^3}$ | $(0, 0)(1, 0)(2, 0)(2, 0)(2, 0)$ |

在 $f_2$ 内嵌套 $f_2(1)$ 相当于 PSS 末尾添加 $(n + 1, 0)$.

| Beta                             |       Ordinal | PSS                              |
|:---------------------------------|--------------:|:---------------------------------|
| $f_2(1)$                         |           $ω$ | $(0, 0)(1, 0)$                   |
| $f_2(1, f_2(1))$                 |         $ω^ω$ | $(0, 0)(1, 0)(2, 0)$             |
| $f_2(1, f_2(1, f_2(1)))$         |     $ω^{ω^ω}$ | $(0, 0)(1, 0)(2, 0)(3, 0)$       |
| $f_2(1, f_2(1, f_2(1, f_2(1))))$ | $ω^{ω^{ω^ω}}$ | $(0, 0)(1, 0)(2, 0)(3, 0)(4, 0)$ |

在 $f_2$ 内嵌套 $f_2(2, f_2(2))$ 相当于 PSS 末尾添加 $4$ 项.

| Beta                                     |           Ordinal | PSS                                                            |
|:-----------------------------------------|------------------:|:---------------------------------------------------------------|
| $f_2(2)$                                 |             $ε_0$ | $(0, 0)(1, 1)$                                                 |
| $f_2(2, f_2(2))$                         |           $ε_0^2$ | $(0, 0)(1, 1)(1, 0)(2, 1)$                                     |
| $f_2(2, f_2(2, f_2(2)))$                 |       $ε_0^{ε_0}$ | $(0, 0)(1, 1)(1, 0)(2, 1)(2, 0)(3, 1)$                         |
| $f_2(2, f_2(2, f_2(2, f_2(2))))$         |     $ε_0^{ε_0^2}$ | $(0, 0)(1, 1)(1, 0)(2, 1)(2, 0)(3, 1)(3, 0)(4, 1)$             |
| $f_2(2, f_2(2, f_2(2, f_2(2, f_2(2)))))$ | $ε_0^{ε_0^{ε_0}}$ | $(0, 0)(1, 1)(1, 0)(2, 1)(2, 0)(3, 1)(3, 0)(4, 1)(4, 0)(5, 1)$ |


做个小结 


$$
\begin{aligned}
f_2(∘, ∘, ∘) &= 1\\ $(0, 0)$
f_2(1, ∘, ∘) &= ω\\  $(0, 0)(1, 0)$
f_2(1, 1, ∘) &= ω^2\\ $(0, 0)(0, 1)(0, 1)$
f_2(1, 1, 1) &= ω^3\\ $(0, 0)(0, 1)(0, 1)(0, 1)$
f_2(2, ∘, ∘) &= ε_0\\ $(0, 0)(1, 1)$
f_2(2, 1, ∘) &= ε_0×ω\\ $(0, 0)(1, 1)(0, 1)$
f_2(2, 2, ∘) &= ε_1\\  $(0, 0)(1, 1)(1, 1)$
f_2(2, 2, 1) &= ε_1×ω\\$(0, 0)(1, 1)(1, 1)(0, 1)$
f_2(2, 2, 2) &= ε_2\\ $(0, 0)(1, 1)(1, 1)(1, 1)$
\end{aligned}
$$

| Beta                                     |           Ordinal | PSS                                                            |
|:-----------------------------------------|------------------:|:---------------------------------------------------------------|

$$
\begin{aligned}
f_3(∘, ∘, ∘) &= ε_{0}\\ $(0, 0)(1, 1)$
f_3(1, ∘, ∘) &= ε_{ω}\\ $(0, 0)(1, 1)(2, 0)$
f_3(1, 1, ∘) &= ε_{ω^2}\\ $(0, 0)(1, 1)(2, 0)(2, 0)$
f_3(1, 1, 1) &= ε_{ω^3}\\$(0, 0)(1, 1)(2, 0)(2, 0)(2, 0)$
\end{aligned}
$$

| Beta                                     |           Ordinal | PSS                                                            |
|:-----------------------------------------|------------------:|:---------------------------------------------------------------|

$$
\begin{aligned}
f_3(f_2(∘, ∘, ∘)) &= ε_{ω}\\ $(0, 0)(1, 1)(2, 0)$
f_3(f_2(1, ∘, ∘)) &= ε_{ω^ω}\\ $(0, 0)(1, 1)(2, 0)(3, 0)$
f_3(f_2(1, 1, ∘)) &= ε_{ω^{ω^2}}\\ $(0, 0)(1, 1)(2, 0)(3, 0)(3, 0)$
f_3(f_2(1, 1, 1)) &= ε_{ω^{ω^3}}\\ $(0, 0)(1, 1)(2, 0)(3, 0)(3, 0)(3, 0)$
f_3(f_2(2, ∘, ∘)) &= ε_{ε_0}\\ $(0, 0)(1, 1)(2, 0)(3, 1)$
f_3(f_2(2, 1, ∘)) &= ε_{ε_0×ω}\\ $(0, 0)(1, 1)(2, 0)(3, 1)(3, 0)$
f_3(f_2(2, 1, 1)) &= ε_{ε_0×ω^2}\\ $(0, 0)(1, 1)(2, 0)(3, 1)(3, 0)(3, 0)$
f_3(f_2(2, 2, ∘)) &= ε_{ε_1}\\ $(0, 0)(1, 1)(2, 0)(3, 1)(3, 1)$
f_3(f_2(2, 2, 1)) &= ε_{ε_1×ω}\\ $(0, 0)(1, 1)(2, 0)(3, 1)(3, 1)(3, 0)$
f_3(f_2(2, 2, 2)) &= ε_{ε_2}\\ $(0, 0)(1, 1)(2, 0)(3, 1)(3, 1)(3, 1)$
\end{aligned}
$$


| Beta                                     |           Ordinal | PSS                                                            |
|:-----------------------------------------|------------------:|:---------------------------------------------------------------|


$$
\begin{aligned}
f_3(∘) &= ε_{ε_0}\\ $(0, 0)(1, 1)$
f_3(f_2(2)) &= ε_{ε_0}\\ $(0, 0)(1, 1)(2, 0)(3, 1)$
f_3(f_2(f_2(2))) &= ε_{ε_{ε_0}}\\ $(0, 0)(1, 1)(2, 0)(3, 1)(3, 0)(4, 1)$
f_3(f_2(f_2(f_2(2)))) &= ε_{ε_{ε_0}}\\ $(0, 0)(1, 1)(2, 0)(3, 1)(3, 0)(4, 1)(4, 0)(5, 1)$
\end{aligned}
$$



$$
\begin{aligned}
f_3(∘, ∘, ∘) &= ε_{0}\\ $(0, 0)(1, 1)$
f_3(1, ∘, ∘) &= ε_{ω}\\ $(0, 0)(1, 1)(2, 0)$
f_3(1, 1, ∘) &= ε_{ω^2}\\ $(0, 0)(1, 1)(2, 0)(2, 0)$
f_3(1, 1, 1) &= ε_{ω^3}\\$(0, 0)(1, 1)(2, 0)(2, 0)(2, 0)$
f_3(2, ∘, ∘) &= ζ_0\\ $(0, 0)(1, 1)(2, 1)$
f_3(2, 1, ∘) &= ζ_ω\\ $(0, 0)(1, 1)(2, 1)(2, 0)$
f_3(2, 1, 1) &= ζ_{ω^2}\\ $(0, 0)(1, 1)(2, 1)(2, 0)(2, 0)$
f_3(2, 2, ∘) &= η_0\\ $(0, 0)(1, 1)(2, 1)(2, 1)$
f_3(2, 2, 1) &= η_ω\\ $(0, 0)(1, 1)(2, 1)(2, 1)(2, 0)$
f_3(2, 2, 2) &= φ(4,0)\\ $(0, 0)(1, 1)(2, 1)(2, 1)(2, 1)$
\end{aligned}
$$


$$
\begin{aligned}
f_3(∘)              &= φ(1, 0)\\ $(0, 0)(1, 1)$
f_3(f_3(1))         &= φ(ω, 0)\\ $(0, 0)(1, 1)(2, 1)(3, 0)$
f_3(f_3(1), f_3(1)) &= φ(ω + 1,0)\\
f_3(f_3(1), f_3(1), f_3(1)) &= φ(ω + 2,0)\\
\end{aligned}
$$

$$
\begin{aligned}
f_3(∘)    &= φ(1, 0)\\
f_3(f_3(2))       &= φ(1, 0, 0)\\
f_3(f_3(2,2))     &= φ(1, 0, 0, 0)\\
f_3(f_3(2,2,2))   &= φ(1, 0, 0, 0, 0)\\
f_3(f_3(2,2,2,2)) &= φ(1, 0, 0, 0, 0, 0)\\
\end{aligned}
$$

其极限为

$$
f_3(f_3(f_3(1))) = φ(1@ω) = ψ(Ω^{Ω^ω})
$$

$$
\begin{aligned}
f_3(∘)                     &= ψ(0)\\
f_3(1)                     &= ψ(ω)\\
f_3(f_3(1))                &= ψ(Ω^ω)\\
f_3(f_3(f_3(1)))           &= ψ(Ω^{Ω^ω})\\
f_3(f_3(f_3(f_3(1))))      &= ψ(Ω^{Ω^{Ω^ω}})\\
f_3(2)                     &= ψ(Ω)\\
f_3(f_3(2))                &= ψ(Ω^Ω)\\
f_3(f_3(f_3(2)))           &= ψ(Ω^{Ω^Ω})\\
f_3(f_3(f_3(f_3(2))))      &= ψ(Ω^{Ω^{Ω^Ω}})\\
\end{aligned}
$$


$$
\begin{aligned}
f_3(∘, ∘, ∘) &= ε_{0}\\
f_3(1, ∘, ∘) &= ε_{ω}\\
f_3(1, 1, ∘) &= ε_{ω^2}\\
f_3(1, 1, 1) &= ε_{ω^3}\\
f_3(2, ∘, ∘) &= φ(2, 0)\\
f_3(2, 1, ∘) &= φ(2, ω)\\
f_3(2, 1, 1) &= φ(2, ω^2)\\
f_3(2, 2, ∘) &= φ(3, 0)\\
f_3(2, 2, 1) &= φ(3, ω)\\
f_3(2, 2, 2) &= φ(4, 0)\\
f_3(3, ∘, ∘) &= ψ(ω)\\
f_3(3, 1, ∘) &= ψ(ψ_1(0)×ω)\\
f_3(3, 1, 1) &= ψ(ψ_1(0)×ω^2)\\
f_3(3, 2, ∘) &= ψ(ψ_1(0)×Ω)\\
f_3(3, 2, 1) &= ψ(ψ_1(0)×Ω)\text{[OCF间断点]}\\
f_3(3, 2, 2) &= ψ(ψ_1(0)×Ω^2)\\
f_3(3, 3, 0) &= ψ(ψ_1(1))\\
f_3(3, 3, 1) &= ψ(ψ_1(1)×ω)\\
f_3(3, 3, 2) &= ψ(ψ_1(1)×Ω)\\
f_3(3, 3, 3) &= ψ(ψ_1(2))\\
\end{aligned}
$$

路尽

$$f_4(1)=ψ(ψ_1(ω))$$

# 元婴期

## 元婴: 自在境

---

$$
\begin{aligned}
f_4(1) &= ψ(ψ_1(ω))\\
f_4(2) &= ψ(ψ_1(Ω))\\
f_4(f_3(3)) &= ψ(ψ_1(ψ_1(1))) \\
f_4(f_3(f_3(3))) &= ψ(ψ_1(ψ_1(ψ_1(1)))) \\
f_4(3, ∘, ∘) &= ψ(Ω_2) \\
f_4(3, 1, ∘) &= ψ(Ω_2) \text{[OCF间断点]}\\
f_4(3, 2, ∘) &= ψ(Ω_2) \text{[OCF间断点]}\\
f_4(3, f_3(f_3(3))) &= ψ(Ω_2×ψ_1(ψ_1(1))) \\
f_4(3, 3, ∘) &= ψ(Ω_2^2) \\
f_4(3, 3, 1) &= ψ(Ω_2^2) \text{[OCF间断点]}\\
f_4(3, 3, 2) &= ψ(Ω_2^2) \text{[OCF间断点]}\\
f_4(3, 3, 3) &= ψ(Ω_2^3) \\
f_4(f_4(1)) &= ψ(Ω_2^ω) \\
f_4(f_4(2)) &= ψ(Ω_2^Ω) \\
f_4(f_4(f_3(f_3(3)))) &= ψ(Ω_2^{ψ_1(Ω_2)}) \\
f_4(f_4(3)) &= ψ(Ω_2^{Ω_2}) \\
f_4(f_4(f_4(3))) &= ψ(Ω_2^{Ω_2^{Ω_2}}) \\
f_4(4, ∘, ∘) &=ψ(ψ_2(1)) \\
f_4(4, 4, ∘) &=ψ(ψ_2(2)) \\
f_4(4, 4, 4) &=ψ(ψ_2(3)) \\
\end{aligned}
$$



---

路尽

$$f_5(1)=ψ(ψ_3(ω))$$

基本上就是

$$
\begin{aligned}
f_n(0)  &=ψ(ψ_{n-2}(0))\\
f_n(1)  &=ψ(ψ_{n-2}(ω))\\
f_n(2)  &=ψ(ψ_{n-2}(Ω))\\
f_n(n)  &=ψ(ψ_{n-1}(1))\\
\end{aligned}
$$

究极路尽

$$f_ω(ω)=ψ(Ω_ω)$$

修到了尽头

00,11 = f2(2)
00,11,10 = f2(2,1)
00,11,21,21 = f2(2,2)

(1, 0) = f2,1
(1, 1) = f2,2
(2, 0) = f3,1
(2, 1) = f3,2
(2, 2) = f3,3
(3, 0) = f4,1
(3, 1) = f4,2
(3, 2) = f4,3
(3, 3) = f4,4

$$
\begin{aligned}
(1, 1) &= ε_0 \\
(2, 0) &= ε_ω \\
(2, 1) &= φ(2, 0) \\
(2, 2) &= ψ(ψ_1(0)) \\
(3, 0) &= ψ(ψ_1(ω)) \\
(3, 1) &= ψ(ψ_1(Ω)) \\
(3, 2) &= ψ(Ω_2) \\
(3, 3) &= ψ(ψ_2(0)) \\
(1, 1, 1) &= ψ(Ω_ω) \\
(2, 0, 0) &= ψ(Ω_ω×ω) \\
(2, 1, 0) &= ψ(Ω_ω×Ω) \\
(2, 1, 1) &= ψ(Ω_{ω^2}) \\
\end{aligned}
$$