$$
\begin{aligned}
ϕ(0) &= ω\\
ϕ(1) &= ω + 1\\
ϕ(2) &= ω + 2\\
ϕ(3) &= ω + 3\\
ϕ(∘) &= ω + ω      &\qquad ∘ &= ϕ(0)\\
ϕ(∘) &= ω + ω + ω  &\qquad ∘ &= ϕ(ϕ(0))\\
ϕ(∙) &= \overbrace{ω + \cdots + ω}^{ω} & ∙ &↦ ϕ(∙)\\
\end{aligned}
$$

此时规定

$$
ϕ(1, 0) = ω × ω = ω ^ 2
$$

---

$$
\begin{aligned}
ϕ(1, 0) &= ω ^ 2\\
ϕ(1, 1) &= ω ^ 2 + 1\\
ϕ(1, 2) &= ω ^ 2 + 2\\
ϕ(1, 3) &= ω ^ 2 + 3\\
ϕ(1, ∘) &= ω ^ 2 + ω     &\qquad ∘ &→ ϕ(0)\\
ϕ(1, ∘) &= ω ^ 2 + ω + 1 &\qquad ∘ &→ ϕ(1)\\
ϕ(1, ∘) &= ω ^ 2 + ω + 2 &\qquad ∘ &→ ϕ(2)\\
ϕ(1, ∘) &= ω ^ 2 + ω + 3 &\qquad ∘ &→ ϕ(3)\\
ϕ(1, ∘) &= ω ^ 2 + ω × 2 &\qquad ∘ &→ ϕ(ϕ(0))\\
ϕ(1, ∘) &= ω ^ 2 + ω × 3 &\qquad ∘ &→ ϕ(ϕ(ϕ(0)))\\
ϕ(1, ∙) &= ω ^ 2 + ω × ω &\qquad ∙ &↦ ϕ(∙)\\
\end{aligned}
$$

也就是说

$$
ϕ(1, ϕ(1, 0))  = ω ^ 2 × 2 
$$

$$
\begin{aligned}
ϕ(1, 0) &= ω ^ 2     \\
ϕ(1, ∘) &= ω ^ 2 × 2  &\qquad ∘ &→ ϕ(1, 0)\\
ϕ(1, ∘) &= ω ^ 2 × 2 + ω &\qquad ∘ &→ ϕ(1, ϕ(0))\\
ϕ(1, ∘) &= ω ^ 2 × 2 + ω × 2 &\qquad ∘ &→ ϕ(1, ϕ(ϕ(0)))\\
ϕ(1, ∘) &= ω ^ 2 × 2 + ω × 2 + 1 &\qquad ∘ &→ ϕ(1, ϕ(ϕ(1)))\\
ϕ(1, ∘) &= ω ^ 2 × 2 + ω × 2 + 2 &\qquad ∘ &→ ϕ(1, ϕ(ϕ(2)))\\
ϕ(1, ∘) &= ω ^ 2 × 3  &\qquad ∘ &→ ϕ(1, ϕ(1, 0))\\
ϕ(1, ∙) &= ω ^ 2 × ω  &\qquad ∙ &↦ ϕ(1, ∙)\\
\end{aligned}
$$

也就是说

$$
ϕ(2, 0)  = ω ^ 3
$$

现在开始卷左边

$$
\begin{aligned}
ϕ(0, 0) &= ω\\
ϕ(1, 0) &= ω ^ 2\\
ϕ(2, 0) &= ω ^ 3\\
ϕ(3, 0) &= ω ^ 4\\
ϕ(∘, 0) &= ω ^ ω  &\qquad ∘ &→ ϕ(0)\\
ϕ(∘, 0) &= ω ^ {ω + 1}  &\qquad ∘ &→ ϕ(1)\\
ϕ(∘, 0) &= ω ^ {ω + 2}  &\qquad ∘ &→ ϕ(2)\\
ϕ(∘, 0) &= ω ^ {ω + 3}  &\qquad ∘ &→ ϕ(3)\\
ϕ(∘, 0) &= ω ^ {ω × 2}  &\qquad ∘ &→ ϕ(ϕ(0))\\
ϕ(∘, 0) &= ω ^ {ω × 3}  &\qquad ∘ &→ ϕ(ϕ(ϕ(0)))\\
ϕ(∘, 0) &= ω ^ {ω ^ 2}  &\qquad ∘ &→ ϕ(1, 0)\\
ϕ(∘, 0) &= ω ^ {ω ^ 2 + 1}  &\qquad ∘ &→ ϕ(1, 1)\\
ϕ(∘, 0) &= ω ^ {ω ^ 2 + ω}  &\qquad ∘ &→ ϕ(1, ϕ(0))\\
ϕ(∘, 0) &= ω ^ {ω ^ 2 × 2}  &\qquad ∘ &→ ϕ(1, ϕ(1, 0))\\
ϕ(∘, 0) &= ω ^ {ω ^ 2 × 2 + 1}  &\qquad ∘ &→ ϕ(1, ϕ(1, 1))\\
ϕ(∙, 0) &= ω ^ {ω ^ 2 × 3}  &\qquad ∙ &↦ ϕ(1, ∙)\\
\end{aligned}
$$


$$
ϕ(ϕ(1, 0), 0)  = ω ^ {ω ^ 2}
$$

这样左侧值的右值达到了极限, 再来看左值:

$$ 
\begin{aligned}
ϕ(∘, 0) &= ω ^ {ω}  &\qquad ∘ &→ ϕ(0, 0)\\
ϕ(∘, 0) &= ω ^ {ω ^ 2}  &\qquad ∘ &→ ϕ(1, 0)\\
ϕ(∘, 0) &= ω ^ {ω ^ 3}  &\qquad ∘ &→ ϕ(2, 0)\\
ϕ(∘, 0) &= ω ^ {ω ^ 4}  &\qquad ∘ &→ ϕ(3, 0)\\
ϕ(∘, 0) &= ω ^ {ω ^ ω}  &\qquad ∘ &→ ϕ(ϕ(0), 0)\\
ϕ(∘, 0) &= ω ^ {ω ^ ω + 1}  &\qquad ∘ &→ ϕ(ϕ(0), 1)\\
ϕ(∘, 0) &= ω ^ {ω ^ ω + 2}  &\qquad ∘ &→ ϕ(ϕ(0), 2)\\
ϕ(∘, 0) &= ω ^ {ω ^ ω + ω}  &\qquad ∘ &→ ϕ(ϕ(0), ϕ(0))\\
ϕ(∘, 0) &= ω ^ {ω ^ {ω × 2}}  &\qquad ∘ &→ ϕ(ϕ(1), 0)\\
ϕ(∘, 0) &= ω ^ {ω ^ {ω × 2} + 1}  &\qquad ∘ &→ ϕ(ϕ(1), 1)\\
ϕ(∘, 0) &= ω ^ {ω ^ {ω × 2} + ω}  &\qquad ∘ &→ ϕ(ϕ(1), ϕ(0))\\
ϕ(∘, 0) &= ω ^ {ω ^ {ω × 2} + ω × 2}  &\qquad ∘ &→ ϕ(ϕ(1), ϕ(1))\\
ϕ(∘, 0) &= ω ^ {ω ^ {ω × 2} + ω × 3}  &\qquad ∘ &→ ϕ(ϕ(1), ϕ(2))\\
ϕ(∘, 0) &= ω ^ {ω ^ {ω × 2} + ω ^ 2}  &\qquad ∘ &→ ϕ(ϕ(1), ϕ(1, 0))\\
ϕ(∘, 0) &= ω ^ {ω ^ {ω × 2} + ω ^ 3}  &\qquad ∘ &→ ϕ(ϕ(1), ϕ(2, 0))\\
ϕ(∘, 0) &= ω ^ {ω ^ ω}        &\qquad ∘ &→ ϕ(ϕ(0), 0)\\
ϕ(∘, 0) &= ω ^ {ω ^ {ω ^ 2}}  &\qquad ∘ &→ ϕ(ϕ(1, 0), 0)\\
ϕ(∘, 0) &= ω ^ {ω ^ {ω ^ ω}}  &\qquad ∘ &→ ϕ(ϕ(ϕ(0), 0), 0)\\
ϕ(∙, 0) &= ω ↗ ω  &\qquad ∙ &→ ϕ(∙, 0)\\
\end{aligned}
$$

这一结果记为 


$$
ϕ(1, 0, 0) = ω ↗ ω = ε_0
$$

$$
\begin{aligned}
ϕ(1, 0, 1) = ε_0 + 1
ϕ(1, 0, ϕ(0)) = ε_0 + ω
ϕ(1, 0, ϕ(1)) = ε_0 + ω \\
ϕ(1, 0, ϕ(1, 0)) = ω ⋅ ω\\
\end{aligned}
$$


ϕ(2, 0) = ω ^ 2

接下来的目标显然是推出 ϕ(3, 0) = ω ^ 3

$$
\begin{aligned}
ϕ(2, 0) = ω ^ 2\\
ϕ(2, 1) = ω ^ 2 + 1\\
ϕ(2, 2) = ω ^ 2 + 2\\
ϕ(2, 3) = ω ^ 2 + 3\\

ϕ(2, ϕ(1, 0)) = ω ^ 2 + ω\\
\end{aligned}
$$

$$
\begin{aligned}
ϕ(2, ϕ(1, 0)) &= ω ^ 2 + ω\\
ϕ(2, ϕ(1, 1)) &= ω ^ 2 + ω + 1\\
ϕ(2, ϕ(1, 2)) &= ω ^ 2 + ω + 2\\
ϕ(2, ϕ(1, 3)) &= ω ^ 2 + ω + 3\\
ϕ(2, ϕ(1, ∘)) &= ω ^ 2 + ω + ω       & ∘ &= ϕ(1, 0)\\
ϕ(2, ϕ(1, ∘)) &= ω ^ 2 + ω + ω + 1 & ∘ &= ϕ(1, 1)\\
ϕ(2, ϕ(1, ∘)) &= ω ^ 2 + ω + ω + 2 & ∘ &= ϕ(1, 2)\\
ϕ(2, ϕ(1, ∘)) &= ω ^ 2 + ω + ω + 3 & ∘ &= ϕ(1, 3)\\
ϕ(2, ϕ(1, ∘)) &= ω ^ 2 + ω + ω + ω & ∙ &= ϕ(1, ϕ(1, 0))\\
ϕ(2, ϕ(1, ∙)) &= ω ^ 2 + \overbrace{ω + \cdots + ω}^{ω} & ∙ &= ϕ(1, ∙)\\
ϕ(2, ϕ(2, 0)) &= ω ^ 2 + ω ^ 2
\end{aligned}
$$

$$
\begin{aligned}
ϕ(2, ϕ(2, 0)) &= ω ^ 2 ⋅ 2\\
ϕ(2, ϕ(2, 1)) &= ω ^ 2 ⋅ 2 + 1\\
ϕ(2, ϕ(2, 2)) &= ω ^ 2 ⋅ 2 + 2\\
ϕ(2, ϕ(2, 3)) &= ω ^ 2 ⋅ 2 + 3\\
ϕ(2, ϕ(2, ∙)) &= ω ^ 2 ⋅ 2 + ω      & ∙ &= ϕ(1, 0)\\
ϕ(2, ϕ(2, ∙)) &= ω ^ 2 ⋅ 2 + ω + 1  & ∙ &= ϕ(1, 1)\\
ϕ(2, ϕ(2, ∙)) &= ω ^ 2 ⋅ 2 + ω + ω & ∙ &= ϕ(1, ϕ(1, 0))\\
ϕ(2, ϕ(2, ∙)) &= ω ^ 2 ⋅ 2 + ω ^ 2 & ∙ &= ϕ(1, ∙)\\
\end{aligned}
$$


$$
\begin{aligned}
ϕ(0, 0) &= 1\\
ϕ(1, 0) &= ω ^ 2\\
ϕ(2, 0) &= ω ^ 2\\
ϕ(3, 0) &= ω ^ 3\\
ϕ(ϕ(1, 0), 0) &= ω ^ ω\\
ϕ(ϕ(1, 0), 1) &= ω ^ ω + 1\\
ϕ(ϕ(1, 0), 2) &= ω ^ ω + 2\\
ϕ(ϕ(1, 0), 2) &= ω ^ ω + 3\\
ϕ(ϕ(1, 0), ∙) &= ω ^ ω + ω     & ∙ &= ϕ(1, 0)\\
ϕ(ϕ(1, 0), ∙) &= ω ^ ω + ω ⋅ 2 & ∙ &= ϕ(2, 0)\\
ϕ(ϕ(1, 0), ∙) &= ω ^ ω + ω ⋅ 3 & ∙ &= ϕ(3, 0)\\
ϕ(ϕ(1, 0), ∙) &= ω ^ ω + ω ^ 2 & ∙ &= ϕ(ϕ(1, 0), 0)\\
\end{aligned}
$$

