学习该定义并总结规律

```
ψZ(0)=1
ψZ[#1][0,#2]=ψZ[#1][#2]
ψZ[#1][#2]=ψZ[#1,#2]
ψZ[#][a+](b+)=ψZ[#][a+](b)+
ψZ[#][a](b)+=ψZ[#][a,b+](b+)
```

前几个值为:




```
ψZ(ω)=ψ(0)
ψZ[ω+1](ω+1)=ψ(0)+1
ψZ[ω+1](ω*2)=ψ(0)+ω
ψZ[ω+1](ω^2)=ψ(0)+ω^2
ψZ[ω+1](ψ(0))=ψ(0)*2
ψZ[ω+1](ψ(0)*2)=ψ(0)*3
ψZ(ω+1)=ψ(0)*ω
ψZ[ω+2](ω+2)=ψ(0)*ω+1
ψZ[ω+2](ω*2)=ψ(0)*ω+ω
ψZ[ω+2](ω^2)=ψ(0)*ω+ω^2
ψZ[ω+2](ψ(0)*ω)=ψ(0)*ω*2
ψZ[ω+2](ψ(0)*ω*2)=ψ(0)*ω*3
ψZ(ω+2)=ψ(0)*ω^2
ψZ(ω+3)=ψ(0)*ω^3



ψZ[ω*2](ω*2)=ψ(0)*ω^ω
ψZ[ω*2,ω*2+1](ω*2+1)=ψ(0)*ω^ω+1
ψZ[ω*2,ω*2+1](ω*3)=ψ(0)*ω^ω+ω
ψZ[ω*2,ω*2+1](ω^2)=ψ(0)*ω^ω+ω^2
ψZ[ω*2](ω*2+1)=ψ(0)*ω^(ω+1)
ψZ[ω*2](ω*2+2)=ψ(0)*ω^(ω+2)
ψZ[ω*2](ω*3)=ψ(0)*ω^(ω*2)
ψZ[ω*2](ω^2)=ψ(0)*ω^(ω^2)
ψZ[ω*2](ψ(0))=ψ(0)^2
ψZ[ω*2,ψ(0)+1](ψ(0)+1)=ψ(0)^2+1
ψZ[ω*2,ψ(0)+1](ψ(0)+ω)=ψ(0)^2+ω
ψZ[ω*2,ψ(0)+1](ψ(0)*2)=ψ(0)^2+ψ(0)
ψZ[ω*2,ψ(0)+1](ψ(0)*3)=ψ(0)^2+ψ(0)*2
ψZ[ω*2,ψ(0)+1](ψ(0)*ω)=ψ(0)^2+ψ(0)*ω
ψZ[ω*2,ψ(0)+1](ψ(0)^2)=ψ(0)^2*2
ψZ[ω*2,ψ(0)+1](ψ(0)^2*2)=ψ(0)^2*3
ψZ[ω*2](ψ(0)+1)=ψ(0)^2*ω
ψZ[ω*2](ψ(0)+2)=ψ(0)^2*ω^2
ψZ[ω*2](ψ(0)+ω)=ψ(0)^2*ω^ω
ψZ[ω*2](ψ(0)*2)=ψ(0)^3
ψZ[ω*2](ψ(0)*3)=ψ(0)^4
ψZ[ω*2](ψ(0)*ω)=ψ(0)^ω
ψZ[ω*2](ψ(0)^2)=ψ(0)^ψ(0)
ψZ[ω*2](ψ(0)^2+1)=ψ(0)^ψ(0)*ω
ψZ[ω*2](ψ(0)^2+ψ(0))=ψ(0)^(ψ(0)+1)
ψZ[ω*2](ψ(0)^2+ψ(0)*2)=ψ(0)^(ψ(0)+2)
ψZ[ω*2](ψ(0)^2*2)=ψ(0)^(ψ(0)*2)
ψZ[ω*2](ψ(0)^3)=ψ(0)^(ψ(0)^2)
ψZ[ω*2](ψ(0)^4)=ψ(0)^(ψ(0)^3)
ψZ[ω*2](ψ(0)^ψ(0))=ψ(0)^ψ(0)^ψ(0)
ψZ(ω*2)=ψ(1)
ψZ(ω*3)=ψ(2)
ψZ(ω*4)=ψ(3)
ψZ[ω^2](ω^2)=ψ(ω)
ψZ[ω^2,ω^2+1](ω^2+1)=ψ(ω)+1
ψZ[ω^2](ω^2+1)=ψ(ω)*ω
ψZ[ω^2](ω^2+2)=ψ(ω)*ω^2
ψZ[ω^2,ω^2+ω](ω^2+ω)=ψ(ω)*ω^ω
ψZ[ω^2,ω^2+ω,ω^2+ω+1](ω^2+ω+1)=ψ(ω)*ω^ω+1
ψZ[ω^2,ω^2+ω](ω^2+ω+1)=ψ(ω)*ω^(ω+1)
ψZ[ω^2,ω^2+ω](ω^2+ω+2)=ψ(ω)*ω^(ω+2)
ψZ[ω^2,ω^2+ω](ω^2*2)=ψ(ω)*ω^(ω^2)
ψZ[ω^2,ω^2+ω](ω^2*3)=ψ(ω)*ω^(ω^2*2)
ψZ[ω^2,ω^2+ω](ω^3)=ψ(ω)*ω^(ω^3)
ψZ[ω^2,ω^2+ω](ω^ω)=ψ(ω)*ω^ω^ω
ψZ[ω^2,ω^2+ω](ψ(0))=ψ(ω)*ψ(0)
ψZ[ω^2,ω^2+ω](ψ(ω))=ψ(ω)^2
ψZ[ω^2,ω^2+ω](ψ(ω)+1)=ψ(ω)^2*ω
ψZ[ω^2,ω^2+ω](ψ(ω)+ω)=ψ(ω)^2*ω^ω
ψZ[ω^2,ω^2+ω](ψ(ω)+ψ(0))=ψ(ω)^2*ψ(0)
ψZ[ω^2,ω^2+ω](ψ(ω)*2)=ψ(ω)^3
ψZ[ω^2,ω^2+ω](ψ(ω)*3)=ψ(ω)^4
ψZ[ω^2,ω^2+ω](ψ(ω)^2)=ψ(ω)^ψ(ω)
ψZ[ω^2,ω^2+ω](ψ(ω)^2+1)=ψ(ω)^ψ(ω)*ω
ψZ[ω^2,ω^2+ω](ψ(ω)^2+ψ(ω))=ψ(ω)^(ψ(ω)+1)
ψZ[ω^2,ω^2+ω](ψ(ω)^2*2)=ψ(ω)^(ψ(ω)*2)
ψZ[ω^2,ω^2+ω](ψ(ω)^3)=ψ(ω)^ψ(ω)^2
ψZ[ω^2,ω^2+ω](ψ(ω)^ω)=ψ(ω)^ψ(ω)^ω
ψZ[ω^2,ω^2+ω](ψ(ω)^ψ(ω))=ψ(ω)^ψ(ω)^ψ(ω)
ψZ[ω^2](ω^2+ω)=ψ(ω+1)
ψZ[ω^2,ω^2+ω+1](ω^2+ω+1)=ψ(ω+1)+1
ψZ[ω^2](ω^2+ω+1)=ψ(ω+1)*ω
ψZ[ω^2](ω^2+ω+2)=ψ(ω+1)*ω^2
ψZ[ω^2,ω^2+ω*2](ω^2+ω*2)=ψ(ω+1)*ω^ω
ψZ[ω^2,ω^2+ω*2,ω^2+ω*2+1](ω^2+ω*2+1)=ψ(ω+1)*ω^ω+1
ψZ[ω^2,ω^2+ω*2](ω^2+ω*2+1)=ψ(ω+1)*ω^(ω+1)
ψZ[ω^2,ω^2+ω*2](ψ(ω+1))=ψ(ω+1)^2
ψZ[ω^2,ω^2+ω*2](ψ(ω+1)^2)=ψ(ω+1)^3
ψZ[ω^2](ω^2+ω*2)=ψ(ω+2)
ψZ[ω^2](ω^2+ω*3)=ψ(ω+3)
ψZ[ω^2](ω^2*2)=ψ(ω*2)
ψZ[ω^2](ω^2*3)=ψ(ω*3)
ψZ[ω^2](ω^3)=ψ(ω^2)
ψZ[ω^2](ω^ω)=ψ(ω^ω)
ψZ[ω^2](ψ(0))=ψ(ψ(0))
ψZ[ω^2](ψ(ψ(0)))=ψ(ψ(ψ(0)))
ψZ(ω^2)=ψ(Ω)
ψZ[ω^2+1](ω^2+1)=ψ(Ω)+1
ψZ[ω^2+1](ψ(Ω))=ψ(Ω)*2
ψZ(ω^2+1)=ψ(Ω)*ω
ψZ(ω^2+2)=ψ(Ω)*ω^2
ψZ[ω^2+ω](ω^2+ω)=ψ(Ω)*ω^ω
ψZ(ω^2+ω)=ψ(Ω+1)
ψZ(ω^2+ω*2)=ψ(Ω+2)
ψZ(ω^2+ω*3)=ψ(Ω+3)
ψZ[ω^2*2](ω^2*2)=ψ(Ω+ω)
ψZ[ω^2*2](ω^2*2+1)=ψ(Ω+ω+1)
ψZ[ω^2*2](ω^2*2+ω)=ψ(Ω+ω*2)
ψZ[ω^2*2](ω^2*2+ω*2)=ψ(Ω+ω*3)
ψZ[ω^2*2](ω^2*3)=ψ(Ω+ω^2)
ψZ[ω^2*2](ω^2*4)=ψ(Ω+ω^2*2)
ψZ[ω^2*2](ω^2*5)=ψ(Ω+ω^2*3)
ψZ[ω^2*2](ω^3)=ψ(Ω+ω^3)
ψZ[ω^2*2](ψ(Ω))=ψ(Ω+ψ(Ω))
ψZ[ω^2*2](ψ(Ω+ψ(Ω)))=ψ(Ω+ψ(Ω+ψ(Ω)))
ψZ(ω^2*2)=ψ(Ω*2)
ψZ(ω^2*3)=ψ(Ω*3)
ψZ[ω^3](ω^3)=ψ(Ω*ω)
ψZ[ω^3](ω^3+1)=ψ(Ω*(ω+1))
ψZ[ω^3](ψ(Ω))=ψ(Ω*ψ(Ω))
ψZ(ω^3)=ψ(Ω^2)
ψZ(ω^3+1)=ψ(Ω^2)*ω
ψZ(ω^3+ω)=ψ(Ω^2+1)
ψZ(ω^3+ω^2)=ψ(Ω^2+Ω)
ψZ(ω^3*2)=ψ(Ω^2*2)
ψZ(ω^3*3)=ψ(Ω^2*3)
ψZ[ω^4](ω^4)=ψ(Ω^2*ω)
ψZ(ω^4)=ψ(Ω^3)
ψZ(ω^5)=ψ(Ω^4)
ψZ[ω^ω](ω^ω)=ψ(Ω^ω)
ψZ[ω^ω](ω^(ω+1))=ψ(Ω^(ω+1))
ψZ[ω^ω](ψ(Ω^ω))=ψ(Ω^ψ(Ω^ω))
ψZ(ω^ω)=ψ(Ω^Ω)
ψZ(ω^ω^ω)=ψ(Ω^Ω^Ω)
ψZ[ψ(0)](ψ(0))=ψ(ψ_1(0))
ψZ[ψ(0),ψ(0)+1](ψ(0)+1)=ψ(ψ_1(0))+1
ψZ[ψ(0)](ψ(0)+1)=ψ(ψ_1(0))*ω
ψZ[ψ(0)](ψ(0)+ω)=ψ(ψ_1(0)+1)
ψZ[ψ(0)](ψ(0)+ω^2)=ψ(ψ_1(0)+Ω)
ψZ[ψ(0)](ψ(0)+ω^3)=ψ(ψ_1(0)+Ω^2)
ψZ[ψ(0)](ψ(0)+ω^ω)=ψ(ψ_1(0)+Ω^Ω)
ψZ[ψ(0)](ψ(0)*2)=ψ(ψ_1(0)*2)
ψZ[ψ(0)](ψ(0)*ω)=ψ(ψ_1(0)*Ω)
ψZ[ψ(0)](ψ(0)*ω^ω)=ψ(ψ_1(0)*Ω^Ω)
ψZ[ψ(0)](ψ(0)^2)=ψ(ψ_1(0)^2)
ψZ[ψ(0)](ψ(0)^ω)=ψ(ψ_1(0)^Ω)
ψZ[ψ(0)](ψ(0)^ω^ω)=ψ(ψ_1(0)^Ω^Ω)
ψZ[ψ(0)](ψ(0)^ψ(0))=ψ(ψ_1(0)^ψ_1(0))
ψZ[ψ(0)](ψ(1))=ψ(ψ_1(1))
ψZ[ψ(0)](ψ(ω))=ψ(ψ_1(Ω))
ψZ[ψ(0)](ψ(ω^ω))=ψ(ψ_1(Ω^Ω))
ψZ[ψ(0)](ψ(ψ(0)))=ψ(ψ_1(ψ_1(0)))
ψZ[ψ(0)](ψ(Ω))=ψ(Ω_2)
ψZ[ψ(0)](ψ(Ω_2))=ψ(Ω_3)
ψZ(ψ(0))=ψ(Ω_ω)
ψZ(ψ(0)+1)=ψ(Ω_ω)*ω
ψZ(ψ(0)+ω)=ψ(Ω_ω+1)
ψZ(ψ(0)+ω^2)=ψ(Ω_ω+Ω)
ψZ(ψ(0)+ω^3)=ψ(Ω_ω+Ω^2)
ψZ(ψ(0)+ω^ω)=ψ(Ω_ω+Ω^Ω)
ψZ[ψ(0)*2](ψ(0)*2)=ψ(Ω_ω+ψ_1(0))
ψZ[ψ(0)*2](ψ(0)*3)=ψ(Ω_ω+ψ_1(0)*2)
ψZ[ψ(0)*2](ψ(ω))=ψ(Ω_ω+ψ_1(Ω))
ψZ[ψ(0)*2](ψ(Ω))=ψ(Ω_ω+ψ_1(Ω_2))
ψZ[ψ(0)*2](ψ(Ω_ω))=ψ(Ω_ω+ψ_1(Ω_ω))
ψZ[ψ(0)*2](ψ(Ω_ω+ψ_1(0)))=ψ(Ω_ω+ψ_2(0))
(ψ(Ω_ω+ψ_2(0)))=ψ(Ω_ω+ψ_3(0))
ψZ(ψ(0)*2)=ψ(Ω_ω*2）
ψZ(ψ(0)*3)=ψ(Ω_ω*3)
ψZ[ψ(0)*ω](ψ(0)*ω)=ψ(Ω_ω*ω)
ψZ[ψ(0)*ω](ψ(0)*(ω+1))=ψ(Ω_ω*(ω+1))
ψZ[ψ(0)*ω](ψ(Ω_ω*ω))=ψ(Ω_ω*ψ(Ω_ω*ω))
ψZ(ψ(0)*ω)=ψ(Ω_ω*Ω)
ψZ(ψ(0)*ω+1)=ψ(Ω_ω*Ω)*ω
ψZ(ψ(0)*ω+ω)=ψ(Ω_ω*Ω+1)
ψZ(ψ(0)*ω+ω^2)=ψ(Ω_ω*Ω+Ω)
ψZ(ψ(0)*ω+ω^ω)=ψ(Ω_ω*Ω+Ω^Ω)
ψZ[ψ(0)*(ω+1)](ψ(0)*(ω+1))=ψ(Ω_ω*Ω+ψ_1(0))
ψZ[ψ(0)*(ω+1)](ψ(0)*(ω+2))=ψ(Ω_ω*Ω+ψ_1(0)*2)
ψZ[ψ(0)*(ω+1)](ψ(Ω_ω))=ψ(Ω_ω*Ω+ψ_1(Ω_ω))
ψZ[ψ(0)*(ω+1)]
(ψ(Ω_ω*2))=ψ(Ω_ω*Ω+ψ_1(Ω_ω*2))
ψZ[ψ(0)*(ω+1)]
(ψ(Ω_ω*ω))=ψ(Ω_ω*Ω+ψ_1(Ω_ω*Ω))
ψZ[ψ(0)*(ω+1)]
(ψ(Ω_ω*ω+ψ_1(0)))=ψ(Ω_ω*Ω+ψ_2(0))
ψZ[ψ(0)*(ω+1)]
(ψ(Ω_ω*ω+ψ_2(0)))=ψ(Ω_ω*Ω+ψ_3(0))
ψZ[ψ(0)*(ω+1)]
(ψ(Ω_ω*(ω+1)))=ψ(Ω_ω*(Ω+1))
ψZ[ψ(0)*(ω+1)](ψ(Ω_ω*ω^2))=ψ(Ω_ω*Ω^2)
ψZ[ψ(0)*(ω+1)](ψ(Ω_ω*ψ(0)))=ψ(Ω_ω*ψ_1(0))
ψZ[ψ(0)*(ω+1)](ψ(Ω_ω*ψ_1(0)))=ψ(Ω_ω*ψ_2(0))
ψZ(ψ(0)*(ω+1))=ψ(Ω_ω^2)
ψZ(ψ(0)*(ω+1)+ω)=ψ(Ω_ω^2+1)
ψZ(ψ(0)*(ω+1)+ω^2)=ψ(Ω_ω^2+Ω)
ψZ[ψ(0)*(ω+2)](ψ(0)*(ω+2))=ψ(Ω_ω^2+ψ_1(0))
ψZ(ψ(0)*(ω+2))=ψ(Ω_ω^2+Ω_ω)
ψZ(ψ(0)*(ω+3))=ψ(Ω_ω^2+Ω_ω*2)
ψZ(ψ(0)*(ω*2))=ψ(Ω_ω^2+Ω_ω*Ω)
ψZ(ψ(0)*(ω*2+1))=ψ(Ω_ω^2*2)
ψZ(ψ(0)*(ω*3+1))=ψ(Ω_ω^2*3)
ψZ(ψ(0)*(ω^2))=ψ(Ω_ω^2*Ω)
ψZ(ψ(0)*(ω^2+1))=ψ(Ω_ω^3)
ψZ(ψ(0)*(ω^3+1))=ψ(Ω_ω^4)
ψZ(ψ(0)*(ω^ω))=ψ(Ω_ω^Ω)
ψZ(ψ(0)*(ω^ω+1))=ψ(Ω_ω^Ω_ω)
ψZ(ψ(0)*(ω^ω^ω+1))=ψ(Ω_ω^Ω_ω^Ω_ω)
ψZ[ψ(0)^2](ψ(0)^2)=ψ(ψ_ω(0))
ψZ[ψ(0)^2](ψ(0)^2+ψ(0))=ψ(ψ_ω(0)+Ω_ω)
ψZ[ψ(0)^2](ψ(0)^2+ψ(0)*ω)=ψ(ψ_ω(0)+Ω_ω*Ω)
ψZ[ψ(0)^2](ψ(0)^2+ψ(0)*(ω+1))=ψ(ψ_ω(0)+Ω_ω^2)
ψZ[ψ(0)^2](ψ(0)^2*2)=ψ(ψ_ω(0)*2)
ψZ[ψ(0)^2](ψ(0)^2*ω)=ψ(ψ_ω(0)*Ω)
ψZ[ψ(0)^2](ψ(0)^2*(ω+1))=ψ(ψ_ω(0)^2)
ψZ[ψ(0)^2](ψ(0)^3)=ψ(ψ_ω(1))
ψZ[ψ(0)^2](ψ(0)^ω)=ψ(ψ_ω(Ω))
ψZ[ψ(0)^2](ψ(0)^(ω+1))=ψ(ψ_ω(ψ_ω(0)))
ψZ[ψ(0)^2](ψ(0)^(ω^2))=ψ(Ω_(ω+1))
ψZ[ψ(0)^2](ψ(0)^(ω^2*2))=ψ(Ω_(ω+1)*2)
ψZ[ψ(0)^2](ψ(0)^(ω^2*3))=ψ(Ω_(ω+1)*3)
ψZ[ψ(0)^2](ψ(0)^(ω^3))=ψ(Ω_(ω+1)*Ω)
ψZ[ψ(0)^2](ψ(0)^(ω^3+1))=ψ(Ω_(ω+1)^2)
ψZ[ψ(0)^2](ψ(0)^(ω^ω+1))=ψ(Ω_(ω+1)^Ω_(ω+1))
ψZ[ψ(0)^2](ψ(0)^ψ(0))=ψ(ψ_(ω+1)(0))
ψZ[ψ(0)^2](ψ(0)^ψ(0)^ψ(0))=ψ(ψ_(ω+1)(1))
ψZ[ψ(0)^2](ψ(0)^ψ(0)^ψ(0)^ψ(0))=ψ(ψ_(ω+1)(2))
ψZ[ψ(0)^2](ψ(1))=ψ(ψ_(ω+1)(ω))
ψZ[ψ(0)^2](ψ(2))=ψ(ψ_(ω+1)(Ω))
ψZ[ψ(0)^2](ψ(3))=ψ(ψ_(ω+1)(Ω_2))
ψZ[ψ(0)^2](ψ(ω))=ψ(ψ_(ω+1)(Ω_ω))
ψZ[ψ(0)^2](ψ(ψ(0)))=ψ(ψ_(ω+1)(ψ_(ω+1)(0)))
ψZ[ψ(0)^2](ψ(Ω))=ψ(Ω_(ω+2))
ψZ[ψ(0)^2](ψ(Ω_2))=ψ(Ω_(ω+3))
ψZ[ψ(0)^2](ψ(Ω_ω))=ψ(Ω_(ω*2))
ψZ[ψ(0)^2](ψ(Ω_(ω+1)))=ψ(Ω_(ω*2+1))
ψZ[ψ(0)^2](ψ(Ω_(ω*2)))=ψ(Ω_(ω*3))
ψZ[ψ(0)^2](ψ(Ω_(ω*3)))=ψ(Ω_(ω*4))
ψZ(ψ(0)^2)=ψ(Ω_(ω^2))
ψZ(ψ(0)^3)=ψ(Ω_(ω^3))
ψZ[ψ(0)^ω](ψ(0)^ω)=ψ(Ω_(ω^ω))
ψZ[ψ(0)^ω](ψ(0)^(ω+1))=ψ(Ω_(ω^(ω+1)))
ψZ[ψ(0)^ω](ψ(0)^(ω^ω))=ψ(Ω_(ω^ω^ω))
ψZ[ψ(0)^ω](ψ(0)^ψ(0))=ψ(Ω_(ψ(0)))
ψZ[ψ(0)^ω](ψ(0)^ψ(0)^ψ(0))=ψ(Ω_(ψ(0)^ψ(0)))
ψZ[ψ(0)^ω](ψ(1))=ψ(Ω_(ψ(1)))
ψZ[ψ(0)^ω](ψ(Ω_(ψ(0))))=ψ(Ω_(ψ(Ω_(ψ(0)))))
ψZ(ψ(0)^ω)=ψ(Ω_Ω)
```

并回答:
1. 什么情况下中括号里的值加 1
2. 什么情况下中括号加一个参数
3. 什么情况下可以省略中括号?
