p(o) = 0
p(1) = 1
p(2) = 2
p(1, 1) = w
p(1, 2) = w + 1
p(1, p(1, 1)) = w + w
p(1, p(1, p(1, 1))) = w × 3
p(2, 1) = w × w
p(2, p(2, 1)) = w^2 + w^2
p(2, p(2, p(2, 1))) = w^2 × 3
p(3, 1) = w^3
p(p(1, 1), 1) = w^w
p(p(1, 1), p(1, 1)) = w^w + w
p(p(1, 1), p(1, p(1, 1))) = w^w + w × 2
p(p(1, 1), p(1, p(1, p(1, 1)))) = w^w + w × 3
p(p(1, 1), p(2, 1)) = w^w + w^2
p(p(1, 1), p(2, p(2, 1))) = w^w + w^2 × 2
p(p(1, 1), p(2, p(2, p(2, 1)))) = w^w + w × 3
p(p(1, 1), p(p(1, 1), 1)) = w^w + w^w
p(p(1, 1), p(p(p(1, 1), 1))) = w^w × 3
p(p(1, 2), 1) = w^w × w
p(p(1, 3), 1) = w^{w+2}
p(p(1, p(1, 1)), 1) = w^{w+w}
p(p(p(1, 1), 1), 1) = w^{w^w}

p(1, 1, 1) = e_0




p(1, 1, 2) = e_0 + 1
p(1, 1, p(1, 1)) = e_0 + w
p(1, 1, p(1, 1, 1)) = e_0 + e_0
p(1, 1, p(1, 1, p(1, 1, 1))) = e_0 × 3


p(1, 2, 1) = e_0 × w
p(1, 2, p(1, 2, 1)) = e_0 × w + e_0 × w
p(1, 2, p(1, 2, p(1, 2, 1))) = e_0 × w × 3


p(1, 3, 1) = e_0 × w ^ 2
p(1, p(1, 1), 1) = e_0 × w ^ w
p(1, p(1, 1, 1), 1) = e_0 × w ^ e_0
p(1, p(1, p(1, 1, 1), 1), 1) = e_0 ^ 3

p(2, 1, 1) = e_0^w

p(2, p(2, 1, 1), 1) = e_0^{w + w}
p(2, p(2, p(2, 1, 1), 1), 1) = e_0^{w × 3}


p(3, 1, 1) = e_0^{w ^ 2}

p(p(1, 1) , 1, 1) = e_0^{w ^ w}





p(1, 1, 1) = e_0

p(1, p(1, 1, 1)) = e_0

p(1, p(1, p(1, 1, 1))) = e_0 * 2

p(2, p(1, 1, 1)) = e_0 * w

p(p(1, 1), p(1, 1, 1)) = e_0 * w × w

p(p(1, 1, 1), p(1, 1, 1)) = e_0 * w^w


p(p(1, p(1, 1, 1)), p(1, 1, 1)) = e_0 * w^w^2

p(p(p(1, 1, 1), 1), p(1, 1, 1)) = e_0 * w^w^w










p(1, 1, 2) = e_0 ^ 2

p(1, 1, p(1, 1)) = e_0 ^ {w}

p(1, 1, p(1, 1, 1)) = e_0 ^ e_0

p(1, 2, 1) = e_1






p(1, 1, 2) = e_0 * 2

p(1, 1, p(1, 1)) = e_0 * w

p(1, 1, p(p(p(1, 1), 1), 1)) = e_0 * w ^ 2


p(1, 1, p(1, 1, 1)) = e_0 * w ^ w


p(1, 1, p(1, 1, 1)) = e_0 * w ^ w ^ w

p(1, 1, p(1, 1, p(1, 1, 1))) = e_0 * w ^ w ^ w

p(1, 2, 1) = e_0 ^ 2

p(1, p(1, 1), 1) = e_0 ^ w


p(1, p(1, 1, 1), 1) = e_0 ^ e_0

p(1, p(1, p(1, 1, 1), 1), 1) = e_0 ^ e_0 ^ e_0

p(2, 1, 1) = e_{1}
p(p(1, 1), 1, 1) = e_{w}
p(p(1, 1, 1), 1, 1) = e_{e_0}



p(1, 1, 1, 1) = z_0;




p(1, 1, 1, 1) = e_1;
p(1, 1, 1, p(1, 1, 1, 1)) = e_1 + e1;
p(1, 1, p(1, 1, 1, 1), 1) = e_1 * e1;
p(1, p(1, 1, 1, 1), 1, 1) = e_1 ^ e1;
p(2, 1, 1, 1) = e_2;
p(p(1, 1), 1, 1, 1) = e_w;

p(1, 1, 1, 1, 1) = z_0;

